heap_lang/lib/barrier/specification.v
@@ -14,9 +14,9 @@ Lemma barrier_spec (heapN N : namespace) :
   heapN ⊥ N →
   ∃ recv send : loc → iProp -n> iProp,
     (∀ P, heap_ctx heapN ⊢ {{ True }} newbarrier #() {{ v,
-                             ∃ l : loc, v = LocV l ★ recv l P ★ send l P }}) ∧
-    (∀ l P, {{ send l P ★ P }} signal (LocV l) {{ _, True }}) ∧
-    (∀ l P, {{ recv l P }} wait (LocV l) {{ _, P }}) ∧
+                             ∃ l : loc, v = #l ★ recv l P ★ send l P }}) ∧
+    (∀ l P, {{ send l P ★ P }} signal #l {{ _, True }}) ∧
+    (∀ l P, {{ recv l P }} wait #l {{ _, P }}) ∧
     (∀ l P Q, recv l (P ★ Q) ={N}=> recv l P ★ recv l Q) ∧
     (∀ l P Q, (P -★ Q) ⊢ (recv l P -★ recv l Q)).
 Proof.
