heap_lang/tactics.v
@@ -32,7 +32,6 @@ Ltac reshape_val e tac :=
     let v1 := reshape_val e1 in let v2 := reshape_val e2 in constr:(PairV v1 v2)
   | InjL ?e => let v := reshape_val e in constr:(InjLV v)
   | InjR ?e => let v := reshape_val e in constr:(InjRV v)
-  | Loc ?l => constr:(LocV l)
   end in let v := go e in first [tac v | fail 2].
 
 Ltac reshape_expr e tac :=
